Add formalization of example 5.1.4 Urzyczyn Sorensen

weak-arithmetics/V0-theory/V0Theory/HilbertStyle.lean
@@ -21,10 +21,11 @@ open Formula
 -- perhaps we should be able to somehow take as axiom a formula,
 -- for which the proof of being of the form A1 / A2 is non-constructive
 -- i.e. have predicate isAxiom. but this is slightly harder in Lean
-inductive Derivable : Formula -> Prop where
-  | ax1 {phi psi} : Derivable $ A1 phi psi
-  | ax2 {phi psi ksi} : Derivable $ A2 phi psi ksi
-  | mp {phi psi} : Derivable (phi ==> psi) -> Derivable phi -> Derivable psi
+inductive Derivable : (List Formula) -> Formula -> Prop where
+| assumption {Γ} {φ} : (φ ∈ Γ) -> Derivable Γ φ
+| axK {Γ} {phi psi} : Derivable Γ $ A1 phi psi
+| axS {Γ} {phi psi ksi} : Derivable Γ $ A2 phi psi ksi
+| mp {Γ} {phi psi} : Derivable Γ (phi ==> psi) -> Derivable Γ phi -> Derivable Γ psi
 
 declare_syntax_cat logic_expr
 
@@ -33,38 +34,53 @@ syntax logic_expr " -> " logic_expr : logic_expr
 syntax "(" logic_expr ")" : logic_expr
 syntax "[Logic| " logic_expr "]" : term
 
-set_option pp.rawOnError true
 elab_rules : term
-  | `([Logic| $i:ident]) => do
-      -- let n := i.getId
-      -- let nameSyntax := Syntax.mkStrLit n.toString
-      let nameExpr ← elabTerm i (some (mkConst ``Name))
-      let res := mkApp (mkConst ``Formula.var) nameExpr
-      return res
-      -- let p <- elabTermEnsuringType (mkIdent i.getId) none
-      -- return mkApp (mkConst ``Formula.var) p
+  | `([Logic| $e:logic_expr]) => elabTerm e none
+  | `(logic_expr| $i:ident) => do
+      let nameExpr ← Term.elabTerm i none
+      return mkApp (mkConst ``Formula.var) nameExpr
 
-  | `([Logic| $p:logic_expr -> $q:logic_expr]) => do
-      -- recursively elaborate the left and right logic_expr parts
+  | `(logic_expr| $p:logic_expr -> $q:logic_expr) => do
       let lhs ← elabTerm (← `([Logic| $p])) none
       let rhs ← elabTerm (← `([Logic| $q])) none
       return mkApp2 (mkConst ``Formula.imp) lhs rhs
 
-  | `([Logic| ($p)]) => do
-      -- elaborate inner expression directly
+  | `(logic_expr| ($p)) => do
       elabTerm (← `([Logic| $p])) none
 
-  -- | stx => do
-  --     logInfo m!"Unsupported syntax in [Logic| ...]: {stx}"
-  --     throwUnsupportedSyntax
+
+partial def extractGammaFromGoal : TacticM Expr := do
+  let goal ← getMainTarget
+  let goal <- whnf goal
+  match goal with
+  | Expr.app (Expr.app (Expr.const name _) gamma) _ =>
+    if name == `HilbertStyle.Derivable then
+      pure gamma
+    else
+      throwError "Goal head constant is not HilbertStyle.Derivable, got: {name}"
+  | _ =>
+    throwError "Goal is not of the form `HilbertStyle.Derivable Γ φ`, got: {goal}"
+
+elab "hilbertDebug" : tactic => do
+  let goal ← getMainTarget
+  let ppGoal := goal.dbgToString
+  logInfo m!"Goal expression: {ppGoal}"
+  -- let goalType ← goal.getType
+  let gamma ← extractGammaFromGoal
+
+  logInfo m!"Gamma: {gamma}"
+
+elab "by_mem" : tactic => do evalTactic (← `(tactic| simp [List.Mem]))
 
 -- Syntax category for Hilbert proof steps
 declare_syntax_cat hilbert_tactic
-syntax "let " ident ":=" logic_expr                                  : hilbert_tactic
-syntax "have" ident ":=" "ax1" logic_expr "," logic_expr                         : hilbert_tactic
-syntax "have" ident ":=" "ax2" logic_expr "," logic_expr "," logic_expr                    : hilbert_tactic
-syntax "have" ident ":=" "mp" ident ident                        : hilbert_tactic
-syntax "conclude " ident                                          : hilbert_tactic
+-- syntax "let " ident ":=" logic_expr : hilbert_tactic
+syntax "have" ident ":" logic_expr "by" "assumption" : hilbert_tactic
+syntax "have" ident ":=" "axK" logic_expr "," logic_expr : hilbert_tactic
+syntax "have" ident ":=" "axS" logic_expr "," logic_expr "," logic_expr : hilbert_tactic
+syntax "have" ident ":=" "mp" ident ident : hilbert_tactic
+syntax "debug" : hilbert_tactic
+syntax "exact " ident : hilbert_tactic
 
 syntax "begin_hilbert " (hilbert_tactic)* : tactic
 
@@ -72,22 +88,43 @@ elab_rules : tactic
   | `(tactic| begin_hilbert $[$tacs:hilbert_tactic]*) => do
     for tacNode in tacs do
       let tac ← match tacNode with
-        | `(hilbert_tactic| let $name:ident := $e:logic_expr) => do
-            let e' <- `([Logic| $e])
-            let phi' <- Lean.Elab.Term.elabTerm e' none
+        -- | `(hilbert_tactic| let $name:ident := $e:logic_expr) => do
+        --     let e' <- `([Logic| $e])
+        --     let phi' <- Lean.Elab.Term.elabTerm e' none
+        --     let phi <- delab phi'
+        --     `(tactic| let $name := $phi)
+        | `(hilbert_tactic| debug) => do
+            `(tactic| hilbertDebug)
+
+        | `(hilbert_tactic| have $name:ident : $phi:logic_expr by assumption) => do
+            -- let e1' <- `([Logic| $e1])
+            -- withoutErrToSorry do
+            let phi' ← Lean.Elab.Term.elabTerm phi none
             let phi <- delab phi'
-            `(tactic| let $name := $phi)
-        | `(hilbert_tactic| have $name:ident := ax1 $e1, $e2) => do
+            let gamma' <- extractGammaFromGoal
+            let gamma <- delab gamma'
+            let goal ← `(Derivable $gamma $phi)
+            -- let goalTy := mkApp2 (mkConst ``Derivable) gamma' phi'
+            -- let byMem ← `(by by_mem)
+            -- let rhs ← mkAppM ``Derivable.assumption #[gamma', phi', ← Lean.Elab.Term.elabTerm byMem (some goalTy)]
+            -- let goal <- getMainGoal
+            -- let fVarId <- goal.assert name goalTy rhs
+
+            `(tactic| have $name : $goal := @Derivable.assumption _ $phi (by by_mem))
+
+        | `(hilbert_tactic| have $name:ident := axK $e1, $e2) => do
             let e1' <- `([Logic| $e1])
             let e2' <- `([Logic| $e2])
             let phi' ← Lean.Elab.Term.elabTerm e1' none
             let psi' ← Lean.Elab.Term.elabTerm e2' none
             let phi <- delab phi'
             let psi <- delab psi'
-            let goal ← `(Derivable (A1 $phi $psi))
-            `(tactic| have $name : $goal := Derivable.ax1)
+            let gamma' <- extractGammaFromGoal
+            let gamma <- delab gamma'
+            let goal ← `(Derivable $gamma (A1 $phi $psi))
+            `(tactic| have $name : $goal := Derivable.axK)
 
-        | `(hilbert_tactic| have $name:ident := ax2 $e1, $e2, $e3) => do
+        | `(hilbert_tactic| have $name:ident := axS $e1, $e2, $e3) => do
             let e1' <- `([Logic| $e1])
             let e2' <- `([Logic| $e2])
             let e3' <- `([Logic| $e3])
@@ -97,21 +134,24 @@ elab_rules : tactic
             let phi <- delab phi'
             let psi <- delab psi'
             let ksi <- delab ksi'
-            `(tactic| have $name : Derivable (A2 $phi $psi $ksi) := Derivable.ax2)
+            let gamma' <- extractGammaFromGoal
+            let gamma <- delab gamma'
+            `(tactic| have $name : Derivable $gamma (A2 $phi $psi $ksi) := Derivable.axS)
 
         | `(hilbert_tactic| have $name:ident := mp $h1 $h2) =>
             `(tactic| have $name := Derivable.mp $h1 $h2)
 
-        | `(hilbert_tactic| conclude $id:ident) =>
+        | `(hilbert_tactic| exact $id:ident) =>
             `(tactic| exact $id)
 
         | _ => throwError m!"Unsupported tactic: {tacNode}"
       withTacticInfoContext tacNode do
-        evalTactic tac
+        withMacroExpansion tacNode tac (evalTactic tac)
+        -- evalTactic tac
 
 
 def a : Name := `a
-variable (φ p q: Name)
+variable (φ ψ ϑ p q: Name)
 
 def phi := [Logic| φ]
 def pphi := [Logic| p -> q]
@@ -122,22 +162,48 @@ def S_type (x y z : Name) := [Logic| (x -> y -> z) -> (x -> y) -> x -> z]
 
 
 -- Urzyczyn, Sorensen: example 5.1.3
-example {φ : Formula} : Derivable (φ ==> φ) := by
-  have a : Derivable $ A2 φ (φ ==> φ) φ := Derivable.ax2
-  have b : Derivable $ A1 φ (φ ==> φ) := Derivable.ax1
+example {φ : Formula} : Derivable [] (φ ==> φ) := by
+  have a : Derivable [] $ A2 φ (φ ==> φ) φ := Derivable.axS
+  have b : Derivable [] $ A1 φ (φ ==> φ) := Derivable.axK
   have c := Derivable.mp a b
-  have d : Derivable $ A1 φ φ := Derivable.ax1
+  have d : Derivable [] $ A1 φ φ := Derivable.axK
   exact Derivable.mp c d
 
-theorem urzyczyn : Derivable [Logic| φ -> φ] := by
+example : Derivable [] [Logic| φ -> φ] := by
   begin_hilbert
-    have a := ax2 φ , φ -> φ, φ
-    have b := ax1 φ, φ -> φ
+    have a := axS φ, φ -> φ, φ
+    have b := axK φ, φ -> φ
     have c := mp a b
-    have d := ax1 φ, φ
+    have d := axK φ, φ
     have e := mp c d
-    conclude e
+    exact e
 
-#check urzyczyn
+-- Urzyczyn, Sorensen: example 5.1.4
+example {φ ψ ϑ: Formula} : Derivable [φ, φ ==> ψ, ψ ==> ϑ] (ϑ) := by
+  have a : Derivable [φ, φ ==> ψ, ψ ==> ϑ] $ φ ==> ψ := Derivable.assumption (by simp [List.Mem])
+  have b : Derivable [φ, φ ==> ψ, ψ ==> ϑ] $ φ := Derivable.assumption (by simp [List.Mem])
+  have c : Derivable [φ, φ ==> ψ, ψ ==> ϑ] $ ψ := Derivable.mp a b
+  have d : Derivable [φ, φ ==> ψ, ψ ==> ϑ] $ ψ ==> ϑ := Derivable.assumption (by simp [List.Mem])
+  have e : Derivable [φ, φ ==> ψ, ψ ==> ϑ] $ ϑ := Derivable.mp d c
+  exact e
+
+syntax "[Logic|" sepBy(logic_expr, ",") "⊢" logic_expr "]": term
+
+elab_rules : term
+  | `([Logic| $assumptions,* ⊢ $goal]) => do
+    let assumpExprs ← assumptions.getElems.mapM (fun stx => elabTerm stx none)
+    let goalExpr ← elabTerm goal none
+    let listExpr <- Lean.Meta.mkListLit (mkConst ``Formula) assumpExprs.toList
+    pure $ mkApp2 (mkConst ``Derivable) listExpr goalExpr
+
+-- Urzyczyn, Sorensen: example 5.1.4
+example : [Logic|φ, φ -> ψ, ψ -> ϑ ⊢  ϑ] := by
+  begin_hilbert
+    have a : φ -> ψ by assumption
+    have b : φ by assumption
+    have c := mp a b
+    have d : ψ -> ϑ by assumption
+    have e := mp d c
+    exact e
 
 end HilbertStyle
